src/core/DY.Core.Trace.State.Properties.fst
@@ -31,13 +31,15 @@ val session_pred_later_:
     (requires 
         tr1 <$ tr2 
       /\ no_set_state_entry_for p sid (tr2 `suffix_after` tr1)
-      /\ sp.session_pred tr1 (get_session_aux p sid tr1) p sid cont
+      /\ session_pred_ tr1 (get_session_aux p sid tr1) p sid cont
     )
-    (ensures sp.session_pred tr2 (get_session_aux p sid tr2) p sid cont)
+    (ensures session_pred_ tr2 (get_session_aux p sid tr2) p sid cont)
 let session_pred_later_ #_ #sp tr1 tr2 p sid cont =
   get_session_aux_same p sid tr1 tr2;
-  let session = get_session_aux p sid tr1 in
-  sp.session_pred_grows tr1 tr2 session p sid cont
+  match get_session_aux p sid tr1 with
+  | None -> ()
+  | Some session ->
+         sp.session_pred_grows tr1 tr2 session p sid cont
 
 let session_pred_later {|invs:protocol_invariants|} = session_pred_later_ #invs.crypto_invs #invs.trace_invs.state_pred
 
@@ -50,21 +52,31 @@ let session_pred_later {|invs:protocol_invariants|} = session_pred_later_ #invs.
 
 val get_state_state_was_set :
   p:principal -> sid:state_id -> tr:trace ->
-  Lemma
-    (requires True)
-    (ensures (
-       let (opt_content, tr_out) = get_state p sid tr in
-       tr == tr_out /\
-       (match opt_content with
-       | None -> True
-       | Some v -> state_was_set tr p sid v
-       )
-      )
-    )
-    [SMTPat (get_state p sid tr)]
+  Lemma 
+  (requires Some? (fst (get_state p sid tr)))
+  (ensures (
+    let (Some cont, tr_out) = get_state p sid tr in
+      tr == tr_out
+    /\ state_was_set tr p sid cont
+  ))
+  [SMTPat (get_state p sid tr)]
 let  get_state_state_was_set p sid tr =
-  normalize_term_spec get_state
+  reveal_opaque (`%get_state) get_state
 
+
+let rec state_was_set_get_state 
+  (p:principal) (sid:state_id) (cont:state_raw) (tr:trace):
+  Lemma 
+  (requires state_was_set tr p sid cont)
+  (ensures Some? (fst (get_state p sid tr)) )
+  =   reveal_opaque (`%get_state) get_state; 
+    match tr with
+    | Nil -> ()
+    | Snoc init (SetState p' sid' cont') ->
+           if p' = p && sid' = sid 
+           then ()
+           else state_was_set_get_state p sid cont init
+    | Snoc init _ -> state_was_set_get_state p sid cont init
 
 let rec get_state_no_set_state_for_on_suffix_after_event
   (tr:trace) (p:principal) (sid:state_id) :
@@ -95,10 +107,10 @@ let rec get_state_no_set_state_for_on_suffix_after_event
 
 let rec get_session_grows (p:principal) (sid:state_id) (tr1 tr2:trace):
   Lemma
-  ( requires tr1 <$ tr2 /\ Some? (get_session p sid tr1)
+  (requires tr1 <$ tr2 /\ Some? (fst (get_session p sid tr1))
   )
   (ensures
-    Some? (get_session p sid tr2)
+    Some? (fst (get_session p sid tr2))
   )
  = reveal_opaque (`%grows) grows; 
    norm_spec [zeta; delta_only [`%prefix]] (prefix);
@@ -110,89 +122,134 @@ let rec get_session_grows (p:principal) (sid:state_id) (tr1 tr2:trace):
      | Snoc init _ -> get_session_grows p sid tr1 init
    )
 
-
-
-let rec get_session_state_was_set (p:principal) (sid:state_id) (tr:trace):
-  Lemma
-  (requires Some? (get_session p sid tr))
-  (ensures exists cont. state_was_set tr p sid cont )
-  = match tr with
-  | Nil -> ()
-  | Snoc init (SetState p' sid' cont') -> (
-         if p' = p && sid' = sid
-         then ()
-         else get_session_state_was_set p sid init
-   )      
-  | Snoc init _ -> 
-        get_session_state_was_set p sid init
-
-
-
 (*** Relations of get_state and get_session ***)
-
-
-
-val get_state_aux_is_last_of_get_session_aux:
-  p:principal -> sid:state_id -> tr:trace ->
-  Lemma 
-    (requires True
-    )
-    (ensures (
-      let session = get_session_aux p sid tr in
-      match get_state_aux p sid tr with
-      | None -> Nil? session
-      | Some st -> Snoc? session /\ (let Snoc _ last = session in st = last)
-    )
-    )
-let rec get_state_aux_is_last_of_get_session_aux p sid tr = 
-  match tr with
-  | Nil -> ()
-  | Snoc init _ -> get_state_aux_is_last_of_get_session_aux p sid init
-
-
-/// relating get_state and get_session
 
 val get_state_is_last_of_get_session:
   p:principal -> sid:state_id -> tr:trace ->
-  Lemma 
-    (requires True
-    )
-    (ensures (
-      let opt_session = get_session p sid tr in
-      let (opt_state, _) = get_state p sid tr in
-      match opt_state with
-      | None -> None? opt_session
-      | Some st -> 
-          Some? opt_session /\ Snoc? (Some?.v opt_session) /\ (let Some (Snoc _ last) = opt_session in st = last)
-    )
-    )
-    [SMTPat (get_session p sid tr); SMTPat (get_state p sid tr)]
-let get_state_is_last_of_get_session p sid tr =
-    reveal_opaque (`%get_state) (get_state);
-    get_state_aux_is_last_of_get_session_aux p sid tr
+  Lemma (
+    let (opt_session, _) = get_session p sid tr in
+    let (opt_state, _) = get_state p sid tr in
+    match opt_state with
+    | None -> None? opt_session
+    | Some st -> 
+        Some? opt_session /\ Snoc? (Some?.v opt_session) 
+        /\ (let Some (Snoc _ last) = opt_session in 
+           st = last
+          )
+  )
+  [SMTPat (get_session p sid tr); SMTPat (get_state p sid tr)]
+let rec get_state_is_last_of_get_session p sid tr =
+  reveal_opaque (`%get_state) (get_state);
+  match tr with
+  | Nil -> ()
+  | Snoc init _ ->  get_state_is_last_of_get_session p sid init
 
+
+let get_state_some_get_session_some (p:principal) (sid:state_id) (tr:trace):
+  Lemma 
+  (requires Some? (fst (get_state p sid tr)))
+  (ensures  Some? (fst (get_session p sid tr)))
+  = ()
+
+
+let rec get_session_some_get_state_some (p:principal) (sid:state_id) (tr:trace):
+  Lemma 
+  (requires Some? (fst (get_session p sid tr)))
+  (ensures Some? (fst (get_state p sid tr)))
+  = 
+    reveal_opaque (`%get_state) get_state;
+    match tr with
+    | Nil -> ()
+    | Snoc init (SetState p' sid' _) ->
+           if p' = p && sid' = sid
+           then ()
+           else get_session_some_get_state_some p sid init
+    | Snoc init _ -> get_session_some_get_state_some p sid init
+
+
+
+let get_session_state_was_set (p:principal) (sid:state_id) (tr:trace):
+  Lemma
+  (requires Some? (fst (get_session p sid tr)))
+  (ensures exists cont. state_was_set tr p sid cont )
+  = get_session_some_get_state_some p sid tr;
+    get_state_state_was_set p sid tr
 
 
 (*** Relation of get_state, get_session and get_full_state ***)
 
 
 /// The main relation:
-/// if the principal has a full state on the trace
-/// and the state id appears in the full state,
-/// then
-/// the entry in full state related to state id is exactly the session
-/// and
-/// the last entry of the session is get state
+/// for any pair (sid, sess) in the full state of a principal [get_full_state p],
+/// we have
+/// * sess is [get_session p sid]
+/// * the last entry of sess is [get_state p sid]
 
+
+let full_state_mem_get_session_get_state_forall (p:principal) (tr:trace):
+  Lemma 
+  (requires Some? (fst (get_full_state p tr)))
+  (ensures (
+     let (Some full_st, _) = get_full_state p tr in
+     forall sid cont. (sid, cont) `List.mem` full_st ==> (
+       let (session_opt, _) = get_session p sid tr in
+       let (state_opt, _) = get_state p sid tr in
+
+         Some? session_opt
+       /\ (let Some sess = session_opt in
+            // content stored in full state related to sid
+            // is [get_session p sid]
+            cont = sess
+          /\ // the content stored is not empty
+            ( Snoc? cont 
+            /\ (let Snoc _ last = cont in
+               // there is a state for p and sid on tr
+               Some? state_opt 
+               /\ // and this state is the last entry in the stored content
+                Some?.v state_opt = last
+              )
+            )
+         )
+       )
+  ))
+=  let (Some full_st, _) = get_full_state p tr in
+   introduce forall sid cont. (sid, cont) `List.mem` full_st ==> (
+     let (session_opt, _) = get_session p sid tr in
+     let (state_opt, _) = get_state p sid tr in
+
+       Some? session_opt
+     /\ (let Some sess = session_opt in
+          cont = sess
+        /\ ( Snoc? cont 
+          /\ (let Snoc _ last = cont in
+               Some? state_opt 
+             /\ Some?.v state_opt = last
+            )
+          )
+       )
+    )
+   with (
+     introduce _ ==> _
+      with _ . (
+        mem_choose_elim 
+          (get_session_aux_indexed tr p) 
+          (zero_to_sid (compute_new_session_id p tr)) 
+          (sid, cont)        
+      )
+   )
+
+// corolloray of the above
+// instantiated for a given state id
 let full_state_some_get_session_get_state (p:principal) (sid:state_id) (tr:trace):
   Lemma 
   (requires
-       Some? (get_full_state p tr)
-     /\ sid `List.mem` (List.map fst (Some?.v (get_full_state p tr)))
+       Some? (fst (get_full_state p tr))
+     /\ // the state id appears as key in the full state
+       sid `List.mem` (List.map fst (Some?.v (fst (get_full_state p tr))))
   )
   (ensures (
-     let Some full_st = get_full_state p tr in
-     let session_opt = get_session p sid tr in
+     let (Some full_st, _) = get_full_state p tr in
+     let (session_opt, _) = get_session p sid tr in
      let (state_opt, _) = get_state p sid tr in
 
      Some? session_opt
@@ -200,48 +257,22 @@ let full_state_some_get_session_get_state (p:principal) (sid:state_id) (tr:trace
         ((sid, sess) `List.mem` full_st)
         /\ ( Snoc? sess 
           /\ (let Snoc _ last = sess in
-             Some? state_opt /\ Some?.v state_opt = last
+               Some? state_opt 
+             /\ Some?.v state_opt = last
             )
           )
        )
    )
   )
-  = let Some full_st = get_full_state p tr in
+  = let (Some full_st, _) = get_full_state p tr in
     FStar.List.Tot.Properties.memP_map_elim fst sid full_st;
-    eliminate exists sess. (sid, sess) `List.mem` full_st 
-    returns Some? (get_session p sid tr) /\ ( (sid, Some?.v (get_session p sid tr)) `List.mem` full_st )
-    with _ . (
-      mem_choose_elim 
-        (get_session_indexed tr p) 
-        (zero_to_sid (compute_new_session_id p tr)) 
-        (sid, sess)
-        )
+    full_state_mem_get_session_get_state_forall p tr
 
 
-
-// corolloray of the above:
-// the entries (si, c) in full state satisfy:
-// c = get_session si
-let full_state_mem_get_session (tr:trace) (p:principal) :
-  Lemma
-  (requires Some? (get_full_state p tr))
-  (ensures (
-    let Some full_st = get_full_state p tr in
-    forall si c. (si, c) `List.mem` full_st  ==> Some c = get_session p si tr
-  ))
-  =     
-  let Some full_st = get_full_state p tr in
-  introduce forall si c. (si, c) `List.mem` full_st ==> Some c = get_session p si tr
-  with(
-    introduce _ ==> _
-    with _ . (
- mem_choose_elim (get_session_indexed tr p) (zero_to_sid (compute_new_session_id p tr)) (si,c);
-  full_state_some_get_session_get_state p si tr
-    )
-  )
 
 (*** Properties of compute_new_session_id ***)
 
+// most of them are needed for [get_full_state_on_growing_traces]
 
 val compute_new_session_id_larger_than_id_on_trace:
   prin:principal -> tr:trace ->
@@ -259,6 +290,8 @@ let rec compute_new_session_id_larger_than_id_on_trace prin tr sess_id state_con
     )
   )
 
+// the result of [compute_new_session_id] stays the same,
+// if there are no more SetState entries for p on the trace
 let rec compute_new_session_id_same (p:principal) (tr1 tr2:trace) :
   Lemma (
     requires
@@ -286,10 +319,15 @@ let rec compute_new_session_id_same (p:principal) (tr1 tr2:trace) :
            compute_new_session_id_same p tr1 init
     )
 
-
-let rec zero_to_sid_mem (bound:state_id) (x :state_id{x.the_id <= bound.the_id}):
-  Lemma ( ensures
-    x `List.mem` (zero_to_sid bound)
+// any number smaller than the bound,
+// appears in [zero_to_sid bound]
+let rec zero_to_sid_mem (bound:state_id) (x :state_id):
+  Lemma
+  (requires
+     x.the_id <= bound.the_id
+  )
+  (ensures
+     x `List.mem` (zero_to_sid bound)
   )
   (decreases bound.the_id)  
   = if bound.the_id = 0
@@ -302,14 +340,16 @@ let rec zero_to_sid_mem (bound:state_id) (x :state_id{x.the_id <= bound.the_id})
         zero_to_sid_mem ({the_id = bound.the_id -1}) x
     end
 
-
+// the opposite of the above:
+// any number in [zero_to_sid bound]
+// is smaller than the bound
 let rec zero_to_sid_mems (bound:state_id) (sid:state_id) :
   Lemma 
   (requires
-    sid `List.mem` (zero_to_sid bound)
+     sid `List.mem` (zero_to_sid bound)
   )
-  ( ensures
-  sid.the_id <= bound.the_id
+  (ensures
+     sid.the_id <= bound.the_id
   )
   (decreases bound.the_id)
   = if bound.the_id = 0
@@ -318,10 +358,10 @@ let rec zero_to_sid_mems (bound:state_id) (sid:state_id) :
       if sid = bound
       then ()
       else (
-     FStar.List.Tot.Properties.append_mem_forall (zero_to_sid {the_id = bound.the_id - 1}) [bound];
-     zero_to_sid_mems ({the_id =bound.the_id - 1}) sid
-     )
-  )
+        FStar.List.Tot.Properties.append_mem_forall (zero_to_sid {the_id = bound.the_id - 1}) [bound];
+        zero_to_sid_mems ({the_id =bound.the_id - 1}) sid
+      )
+    )
 
 let rec compute_new_session_id_grows (p:principal) (tr1 tr2:trace):
   Lemma 
@@ -342,82 +382,105 @@ let rec compute_new_session_id_grows (p:principal) (tr1 tr2:trace):
 
 
 
-(*** More Relation on get_session and get_full_state ***)
+(*** More Relation on get_state, get_session and get_full_state ***)
 
-let get_session_some_full_state_some (p:principal) (sid:state_id) (tr:trace):
+let get_session_some_get_full_state_some (p:principal) (sid:state_id) (tr:trace):
   Lemma 
-  ( requires Some? (get_session p sid tr)
-  )
-  (ensures Some? (get_full_state p tr)
+  (requires Some? (fst (get_session p sid tr)))
+  (ensures Some? (fst (get_full_state p tr)) 
+  // /\  sid `List.mem` (List.map fst (Some?.v (fst (get_full_state p tr))))
   )
   =
     get_session_state_was_set p sid tr;
     eliminate exists cont . state_was_set tr p sid cont
-    returns Some? (get_full_state p tr)
+    returns Some? (fst (get_full_state p tr))
     with _ .
         compute_new_session_id_larger_than_id_on_trace p tr sid cont
 
 
+val get_state_some_get_full_state_some:
+  tr:trace -> p:principal -> sid:state_id ->
+  Lemma 
+  (requires Some? (fst (get_state p sid tr)))
+  (ensures  Some? (fst (get_full_state p tr)))
+let get_state_some_get_full_state_some tr p sid  =  
+  get_session_some_get_full_state_some p sid tr
+
+
+// funktioniert noch nicht so richtig
+// let ad (p:principal) (sid:state_id) (tr:trace):
+//   Lemma (
+//       Some? (fst (get_state p sid tr )) <==> Some? (fst (get_session p sid tr))
+//     /\ Some? (fst (get_session p sid tr)) <==> (Some? (fst (get_full_state p tr)) /\ sid `List.mem` (List.map fst (Some?.v (fst (get_full_state p tr)))))
+//   )
+// = 
+//   FStar.Classical.move_requires_3 get_state_some_get_session_some p sid tr;
+//   FStar.Classical.move_requires_3 get_session_some_get_state_some p sid tr;
+//   FStar.Classical.move_requires_3 get_session_some_get_full_state_some p sid tr;
+//   FStar.Classical.move_requires_3 full_state_some_get_session_get_state p sid tr;
+//   ()
+  
 (*** Properties of get_full_state ***)
 
+// the full state stays the same 
+// if there are no more SetState entries for p
 let get_full_state_same (p:principal) (tr1:trace) (tr2:trace):
   Lemma
   (requires
-      tr1 <$ tr2 /\ 
-      no_set_state_entry_for_p p (tr2 `suffix_after` tr1)
-    )
-  (ensures get_full_state p tr1 = get_full_state p tr2)
-= introduce forall sid. get_session_indexed tr1 p sid = get_session_indexed tr2 p sid
+     tr1 <$ tr2 /\ 
+     no_set_state_entry_for_p p (tr2 `suffix_after` tr1)
+  )
+  (ensures fst (get_full_state p tr1) = fst (get_full_state p tr2))
+= introduce forall sid. get_session_aux_indexed tr1 p sid = get_session_aux_indexed tr2 p sid
   with (
     reveal_opaque (`%get_session) get_session; 
     get_session_aux_same p sid tr1 tr2
   ); 
   compute_new_session_id_same p tr1 tr2;
   choose_equals
-    (get_session_indexed tr1 p) 
-    (get_session_indexed tr2 p) 
+    (get_session_aux_indexed tr1 p) 
+    (get_session_aux_indexed tr2 p) 
     (zero_to_sid (compute_new_session_id p tr1))
 
 
 let full_state_fst_zero_to_sid (tr:trace) (p:principal):
   Lemma
-  ( requires Some? (get_full_state p tr)
-  )
+  (requires Some? (fst (get_full_state p tr)))
   (ensures (
-    let Some full_st = get_full_state p tr in
-    let next_sid = compute_new_session_id p tr in
-    (List.map fst (full_st)) `List.subset` (zero_to_sid next_sid)
-   )
-  )
+     let (Some full_st,  _) = get_full_state p tr in
+     let next_sid = compute_new_session_id p tr in
+     (List.map fst (full_st)) `List.subset` (zero_to_sid next_sid)
+  ))
   =
-    let Some full_st = get_full_state p tr in
+    let (Some full_st, _) = get_full_state p tr in
     let next_sid = compute_new_session_id p tr in
-  introduce forall sid. sid `List.mem` (List.map fst full_st) ==> sid `List.mem` (zero_to_sid next_sid)
-  with (
-    introduce _ ==> _
-    with _ . (
-      FStar.List.Tot.Properties.memP_map_elim fst sid full_st;
-      eliminate exists sess. (sid, sess) `List.mem` full_st
-      returns _
+    introduce forall sid. sid `List.mem` (List.map fst full_st) ==> sid `List.mem` (zero_to_sid next_sid)
+    with (
+      introduce _ ==> _
       with _ . (
-      mem_choose_elim (get_session_indexed tr p) (zero_to_sid next_sid) (sid,sess)    
+        FStar.List.Tot.Properties.memP_map_elim fst sid full_st;
+        eliminate exists sess. (sid, sess) `List.mem` full_st
+        returns _
+        with _ . (
+          mem_choose_elim (get_session_aux_indexed tr p) (zero_to_sid next_sid) (sid,sess)    
+        )
       )
     )
-  )
 
+// a sid stored in a full state remains in the full state when the trace grows
 let get_full_state_on_growing_traces (p:principal) (tr1 tr2:trace) (sid:state_id):
   Lemma 
   (requires
-      tr1 <$ tr2
-    /\ Some? (get_full_state p tr1)
-    /\ sid `List.mem` (List.map fst (Some?.v (get_full_state p tr1)))
+       tr1 <$ tr2
+     /\ Some? (fst (get_full_state p tr1))
+     /\ sid `List.mem` (List.map fst (Some?.v (fst (get_full_state p tr1))))
   )
   (ensures
-    Some? (get_full_state p tr2) /\    
-    sid `List.mem` (List.map fst (Some?.v (get_full_state p tr2)))
+       Some? (fst (get_full_state p tr2))    
+     /\ sid `List.mem` (List.map fst (Some?.v (fst (get_full_state p tr2))))
   )
   = 
-  let Some full_st1 = get_full_state p tr1 in
+  let (Some full_st1, _) = get_full_state p tr1 in
   let new_sid1 = compute_new_session_id p tr1 in
   let new_sid2 = compute_new_session_id p tr2 in
   compute_new_session_id_grows p tr1 tr2;
@@ -429,44 +492,52 @@ let get_full_state_on_growing_traces (p:principal) (tr1 tr2:trace) (sid:state_id
 
   full_state_some_get_session_get_state p sid tr1;
   get_session_grows p sid tr1 tr2;
-  let Some sess2 = get_session p sid tr2 in
-  get_session_some_full_state_some p sid tr2;
-  let Some full_st2 = get_full_state p tr2 in
-  mem_choose (get_session_indexed tr2 p) sids2 sid;
+  let (Some sess2, _) = get_session p sid tr2 in
+  get_session_some_get_full_state_some p sid tr2;
+  let (Some full_st2, _) = get_full_state p tr2 in
+  mem_choose (get_session_aux_indexed tr2 p) sids2 sid;
   FStar.List.Tot.Properties.memP_map_intro fst (sid, sess2) full_st2
    
 (*** More Relations on get_state and get_full_state ***)
 
+let state_was_set_full_state_some (tr:trace) (p:principal) (sid:state_id) (cont:bytes):
+  Lemma 
+  (requires state_was_set tr p sid cont)
+  (ensures Some? (fst (get_full_state p tr)))
+  [SMTPat (state_was_set tr p sid cont)]
+  = 
+  state_was_set_get_state p sid cont tr;
+  get_state_some_get_full_state_some tr p sid
 
 let rec state_was_set_full_state (tr:trace) (p:principal) (sid:state_id) (cont:bytes):
   Lemma
-  (requires
-    state_was_set tr p sid cont
-  )
-  (ensures
-    Some? (get_full_state p tr) 
-    /\ sid `List.mem` (List.map fst (Some?.v (get_full_state p tr)))
-  )
-= match tr with
+  (requires state_was_set tr p sid cont )
+  (ensures (
+     sid `List.mem` (List.map fst (Some?.v (fst (get_full_state p tr))))
+  ))
+= 
+  match tr with
   | Nil -> ()
   | Snoc init (SetState p' sid' cont') ->
       if p' = p 
         then ( 
-        if sid' = sid
-        then (
-          compute_new_session_id_larger_than_id_on_trace p tr sid cont';
-          zero_to_sid_mem (compute_new_session_id p tr) sid;
-          assert(Some? (get_session p sid tr));
-          let f = get_session_indexed tr p in
-          let sids = (zero_to_sid (compute_new_session_id p tr)) in
-          let Some full_st = get_full_state p tr in
-          mem_choose f sids sid;
-          FStar.List.Tot.Properties.memP_map_intro fst (sid, Some?.v (get_session p sid tr)) full_st
+          if sid' = sid
+          then (
+            compute_new_session_id_larger_than_id_on_trace p tr sid cont';
+            zero_to_sid_mem (compute_new_session_id p tr) sid;
+            assert(Some? (fst (get_session p sid tr)));
+            let f = get_session_aux_indexed tr p in
+            let sids = (zero_to_sid (compute_new_session_id p tr)) in
+            let (Some full_st, _) = get_full_state p tr in
+            mem_choose f sids sid;
+            FStar.List.Tot.Properties.memP_map_intro fst (sid, Some?.v (fst (get_session p sid tr))) full_st
           )
           else (
-          init_is_prefix tr;
-          state_was_set_full_state init p sid cont;
-          get_full_state_on_growing_traces p init tr sid
+            init_is_prefix tr;
+            state_was_set_full_state init p sid cont;
+            state_was_set_full_state_some init p sid cont;
+
+            get_full_state_on_growing_traces p init tr sid
           )
         )
         else (
@@ -479,37 +550,23 @@ let rec state_was_set_full_state (tr:trace) (p:principal) (sid:state_id) (cont:b
      get_full_state_same p init tr;
      state_was_set_full_state init p sid cont
 
-val get_state_get_full_state:
-  tr:trace -> p:principal -> sid:state_id ->
-  Lemma 
-  ( requires Some? (fst (get_state p sid tr))
-  )
-  (ensures Some? (get_full_state p tr)
-  )
-let get_state_get_full_state tr p sid  =  
-  let (Some state, _) = get_state p sid tr in
-  get_state_state_was_set p sid tr;
-  state_was_set_full_state tr p sid state
-
 val get_state_appears_in_full_state :
   tr:trace -> p:principal -> sid:state_id ->
   Lemma
-  (requires
-       Some? (fst (get_state p sid tr))
-  )
+  (requires Some? (fst (get_state p sid tr)))
   (ensures (
-    let (Some state, _) = get_state p sid tr in
-    get_state_get_full_state tr p sid;
-    let Some full_state = get_full_state p tr in
-    
-    exists init. (sid, Snoc init state) `List.mem` full_state 
-  )
-  )
+     let (Some state, _) = get_state p sid tr in
+   
+     get_state_some_get_full_state_some tr p sid;
+     let (Some full_state, _) = get_full_state p tr in
+
+     exists init. (sid, Snoc init state) `List.mem` full_state 
+  ))
 let get_state_appears_in_full_state  tr p sid =
   let (Some state, _) = get_state p sid tr in
 
-  get_state_get_full_state tr p sid;
-  let Some full_state = get_full_state p tr in
+  get_state_some_get_full_state_some tr p sid;
+  let (Some full_state, _) = get_full_state p tr in
   
   state_was_set_full_state tr p sid state;
   FStar.List.Tot.Properties.memP_map_elim fst sid full_state;
